qa/lean/Ragu.lean
@@ -10,7 +10,8 @@ import Ragu.Instances.Element.Square
 import Ragu.Instances.Element.Alloc
 import Ragu.Instances.Element.AllocSquare
 import Ragu.Instances.Element.DivNonzero
-import Ragu.Instances.Element.Fold
+import Ragu.Instances.Element.FoldN3
+import Ragu.Instances.Element.FoldN7
 import Ragu.Instances.Element.EnforceRootOfUnityK2
 import Ragu.Instances.Element.EnforceRootOfUnityK5
 import Ragu.Instances.Element.EnforceZero
