qa/lean/Ragu/Instances/Element/FoldN3.lean
@@ -1,0 +1,53 @@
+import Ragu.Circuits.Element.Fold
+import Ragu.Instances.Autogen.Element.FoldN3
+import Ragu.Core
+
+namespace Ragu.Instances.Element.FoldN3
+open Ragu.Instances.Autogen.Element.FoldN3
+
+def deserializeInput (input : Vector (Expression (F p)) inputLen)
+    : Var (Circuits.Element.Fold.Input 3) (F p) :=
+  { xs := #v[input[0], input[1], input[2]], s := input[3] }
+
+def serializeOutput (output : Var field (F p)) : Vector (Expression (F p)) 1 :=
+  #v[output]
+
+def formal_instance : Core.Statements.FormalInstance where
+  p
+  exportedOperations
+  exportedOutput
+
+  deserializeInput
+  serializeOutput
+
+  reimplementation := (Circuits.Element.Fold.circuit 3).isGeneralFormalCircuit.toWithHint
+
+  same_constraints := by
+    intro input
+    simp [Core.Statements.FlatOperation.eraseCompute, List.map,
+      Operations.toFlat, circuit_norm,
+      FormalCircuit.isGeneralFormalCircuit,
+      GeneralFormalCircuit.toWithHint,
+      GeneralFormalCircuit.WithHint.toSubcircuit, FormalCircuit.toSubcircuit,
+      deserializeInput, exportedOperations,
+      Circuits.Element.Fold.circuit,
+      Circuits.Element.Fold.elaborated,
+      Circuits.Element.Fold.main,
+      Circuits.Element.Fold.hornerStep,
+      Circuits.Element.Mul.circuit, Circuits.Element.Mul.elaborated, Circuits.Element.Mul.main]
+    rfl
+  same_output := by
+    intro input
+    simp [circuit_norm,
+      FormalCircuit.isGeneralFormalCircuit,
+      GeneralFormalCircuit.toWithHint,
+      GeneralFormalCircuit.WithHint.toSubcircuit, FormalCircuit.toSubcircuit,
+      deserializeInput, serializeOutput,
+      Circuits.Element.Fold.circuit,
+      Circuits.Element.Fold.elaborated,
+      Circuits.Element.Fold.main,
+      Circuits.Element.Fold.hornerStep,
+      Circuits.Element.Mul.circuit, Circuits.Element.Mul.elaborated, Circuits.Element.Mul.main]
+    rfl
+
+end Ragu.Instances.Element.FoldN3
